Revert "fix(proofs-lib/fstar): make type implicits on typeclasses"
This reverts commit 253fb96ada948361b481dd7e525ce5a0276323e7.

proof-libs/fstar/core/Core.Cmp.fsti
@@ -1,11 +1,11 @@
 module Core.Cmp
 open Rust_primitives
 
-class min_tc #t = {
+class min_tc t = {
   min: t -> t -> t
 }
 
-instance min_inttype (#t:inttype): min_tc #(int_t t) = {
+instance min_inttype (#t:inttype): min_tc (int_t t) = {
   min = fun a b -> if a <. b then a else b
 }
 
@@ -14,26 +14,26 @@ type t_Ordering =
   | Ordering_Equal : t_Ordering
   | Ordering_Greater : t_Ordering
 
-class t_Ord (#v_Self: Type) = {
+class t_Ord (v_Self: Type) = {
   f_cmp:v_Self -> v_Self -> t_Ordering;
   // f_max:v_Self -> v_Self -> v_Self;
   // f_min:v_Self -> v_Self -> v_Self;
   // f_clamp:v_Self -> v_Self -> v_Self -> v_Self
 }
 
-class t_PartialEq (#v_Self: Type) (#v_Rhs: Type) = {
+class t_PartialEq (v_Self: Type) (v_Rhs: Type) = {
   // __constraint_1069563329_t_PartialEq:t_PartialEq v_Self v_Rhs;
   f_eq:v_Self -> v_Rhs -> bool;
   f_ne:v_Self -> v_Rhs -> bool
 }
 
-instance all_eq (a: eqtype): t_PartialEq #a #a = {
+instance all_eq (a: eqtype): t_PartialEq a a = {
   f_eq = (fun x y -> x = y);
   f_ne = (fun x y -> x <> y);
 }
 
-class t_PartialOrd (#v_Self: Type) (#v_Rhs: Type) = {
-  __constraint_Rhs_t_PartialEq:t_PartialEq #v_Self #v_Rhs;
+class t_PartialOrd (v_Self: Type) (v_Rhs: Type) = {
+  __constraint_Rhs_t_PartialEq:t_PartialEq v_Self v_Rhs;
   // __constraint_Rhs_t_PartialOrd:t_PartialOrd v_Self v_Rhs;
   f_partial_cmp:v_Self -> v_Rhs -> Core.Option.t_Option t_Ordering;
   // f_lt:v_Self -> v_Rhs -> bool;
@@ -47,7 +47,7 @@ type t_Reverse t = | Reverse of t
 let impl__then x y = x
 
 [@FStar.Tactics.Typeclasses.tcinstance]
-val ord_u64: t_Ord #u64
+val ord_u64: t_Ord u64
 
 [@FStar.Tactics.Typeclasses.tcinstance]
-val ord_reverse t {| t_Ord #t |}: t_Ord #(t_Reverse t)
+val ord_reverse t {| t_Ord t |}: t_Ord (t_Reverse t)
