proof-libs/fstar/core/Core.Iter.Traits.Collect.fst
@@ -1,14 +1,14 @@
 module Core.Iter.Traits.Collect
 
-class into_iterator #self = {
+class into_iterator self = {
   f_IntoIter: Type0;
   // f_Item: Type0;
   f_into_iter: self -> f_IntoIter;
 }
 
-let t_IntoIterator #self = into_iterator #self
+let t_IntoIterator = into_iterator
 
-unfold instance impl t {| Core.Iter.Traits.Iterator.iterator #t |}: into_iterator #t = {
+unfold instance impl t {| Core.Iter.Traits.Iterator.iterator t |}: into_iterator t = {
   f_IntoIter = t;
   f_into_iter = id;
 }
