proof-libs/fstar/core/Core.Convert.fst
@@ -2,13 +2,13 @@
 module Core.Convert
 open Rust_primitives
 
-class try_into_tc #self #t = {
+class try_into_tc self t = {
   [@@@FStar.Tactics.Typeclasses.no_method]
   f_Error: Type0;
   f_try_into: self -> Core.Result.t_Result t f_Error
 }
 
-instance impl_6 (t: Type0) (len: usize): try_into_tc #(t_Slice t) #(t_Array t len) = {
+instance impl_6 (t: Type0) (len: usize): try_into_tc (t_Slice t) (t_Array t len) = {
   f_Error = Core.Array.t_TryFromSliceError;
   f_try_into = (fun (s: t_Slice t) -> 
     if Core.Slice.impl__len s = len
@@ -18,26 +18,26 @@ instance impl_6 (t: Type0) (len: usize): try_into_tc #(t_Slice t) #(t_Array t le
 }
 
 
-instance impl_6_refined (t: Type0) (len: usize): try_into_tc #(s: t_Slice t {Core.Slice.impl__len s == len}) #(t_Array t len) = {
+instance impl_6_refined (t: Type0) (len: usize): try_into_tc (s: t_Slice t {Core.Slice.impl__len s == len}) (t_Array t len) = {
   f_Error = Core.Array.t_TryFromSliceError;
   f_try_into = (fun (s: t_Slice t {Core.Slice.impl__len s == len}) -> 
     Core.Result.Result_Ok (s <: t_Array t len)
   )
 }
 
-class t_Into #self #t = {
+class t_Into self t = {
   f_into_pre: self -> bool;
   f_into_post: self -> t -> bool;
   f_into: self -> t;
 }
 
-class t_From #self #t = {
+class t_From self t = {
   f_from_pre: t -> bool;
   f_from_post: t -> self -> bool;
   f_from: t -> self;
 }
 
-class t_TryFrom #self #t = {
+class t_TryFrom self t = {
   [@@@FStar.Tactics.Typeclasses.no_method]
   f_Error: Type0;
   f_try_from_pre: t -> bool;
@@ -47,26 +47,26 @@ class t_TryFrom #self #t = {
 
 instance integer_into
   (t:inttype) (t':inttype { minint t >= minint t' /\ maxint t <= maxint t' })
-  : t_From #(int_t t') #(int_t t)
+  : t_From (int_t t') (int_t t)
   = {
       f_from_pre = (fun _ -> true);
       f_from_post = (fun _ _ -> true);
       f_from = (fun (x: int_t t) -> Rust_primitives.Integers.cast #t #t' x);
     }
 
-instance into_from_from a b {| t_From #a #b |}: t_Into #b #a = {
+instance into_from_from a b {| t_From a b |}: t_Into b a = {
   f_into_pre = (fun _ -> true);
   f_into_post = (fun _ _ -> true);
   f_into = (fun x -> f_from x)
 }
 
-instance from_id a: t_From #a #a = {
+instance from_id a: t_From a a = {
   f_from_pre = (fun _ -> true);
   f_from_post = (fun _ _ -> true);
   f_from = (fun x -> x)
 }
 
-class t_AsRef #self #t = {
+class t_AsRef self t = {
   f_as_ref_pre: self -> bool;
   f_as_ref_post: self -> t -> bool;
   f_as_ref: self -> t;
