proof-libs/fstar/core/Core.Default.fsti
@@ -1,5 +1,5 @@
 module Core.Default
 
-class t_Default (#t: Type0) = {
+class t_Default (t: Type0) = {
   v_default: unit -> t;
 }
