proof-libs/fstar/core/Core.Marker.fst
@@ -1,19 +1,19 @@
 module Core.Marker
 
-class t_Sized (#h: Type) = {
+class t_Sized (h: Type) = {
   dummy_field: unit
 }
 
 (** we consider everything to be sized *)
-instance t_Sized_all t: t_Sized #t = {
+instance t_Sized_all t: t_Sized t = {
   dummy_field = ()
 }
 
-class t_Copy (#h: Type) = {
+class t_Copy (h: Type) = {
   dummy_copy_field: unit
 }
 
 (** we consider everything to be copyable *)
-instance t_Copy_all t: t_Copy #t = {
+instance t_Copy_all t: t_Copy t = {
   dummy_copy_field = ()
 }
