proof-libs/fstar/core/Core.Ops.Index.IndexMut.fst
@@ -1,13 +1,13 @@
 module Core.Ops.Index.IndexMut
 
-class t_IndexMut #t_Self #t_Idx = {
+class t_IndexMut t_Self t_Idx = {
   f_Input: Type0;
   in_range: t_Self -> t_Idx -> Type0;
   f_index_mut: s:t_Self -> i:t_Idx{in_range s i} -> v:f_Input -> t_Self;
 }
 
 open Rust_primitives
-instance impl__index_mut t l n: t_IndexMut #(t_Array t l) #(int_t n)
+instance impl__index_mut t l n: t_IndexMut (t_Array t l) (int_t n)
   = { f_Input = t;
       in_range = (fun (s: t_Array t l) (i: int_t n) -> v i >= 0 && v i < v l);
       f_index_mut = (fun s i x -> Seq.upd s (v i) x);
